theories/Substitution/Introductions/Lambda.v
@@ -79,9 +79,10 @@ Proof.
   assert [Δ |- (tLambda F t)[σ] : (tProd F G)[σ]] by (escape; cbn; gen_typing).
   exists (tLambda F t)[σ]; intros; cbn in *.
   + now eapply redtmwf_refl.
-  + constructor;  unshelve eapply escapeEq, reflLRTyEq; [|tea].
+  + constructor; cbn; intros.
+    apply reflLRTyEq.
   + eapply convtm_eta; tea.
-    1,2: constructor; unshelve eapply escapeEq, reflLRTyEq; [|tea].
+    1,2: constructor; eapply escapeEq, reflLRTyEq.
     assert (eqσ : forall Z, Z[up_term_term σ] = Z[up_term_term σ]⟨upRen_term_term S⟩[(tRel 0) ..])
     by (intro; bsimpl; cbn; now rewrite rinstInst'_term_pointwise).
     assert [Δ,, F[σ] |-[ ta ] tApp (tLambda F[σ] t[up_term_term σ])⟨S⟩ (tRel 0) ⤳*  t[up_term_term σ]⟨upRen_term_term S⟩[(tRel 0)..] : G[up_term_term σ]].
@@ -142,13 +143,14 @@ Proof.
     eapply LRTyEqSym. eapply (validTyExt VΠFG); tea.
     Unshelve. 2: now eapply validTy.
   - refold; cbn; escape.
-    eapply convtm_eta; tea.
-    2,4: constructor; first [assumption|now eapply lrefl].
+    eapply convtm_eta; refold; tea.
+    2,4: constructor; first [assumption|now eapply lrefl|idtac].
     + gen_typing.
-    + eapply ty_conv; [gen_typing| now symmetry].
+    + eapply ty_conv; [now eapply ty_lam|].
+      symmetry; now eapply convty_prod.
     + assert (eqσ : forall σ Z, Z[up_term_term σ] = Z[up_term_term σ]⟨upRen_term_term S⟩[(tRel 0) ..])
       by (intros; bsimpl; cbn; now rewrite rinstInst'_term_pointwise).
-      eapply convtm_exp. 
+      eapply convtm_exp.
       * rewrite (eqσ σ G). eapply redtm_beta.
         -- renToWk; eapply wft_wk; tea; gen_typing.
         -- renToWk; eapply ty_wk; tea.
@@ -237,6 +239,17 @@ Proof.
   * unshelve eapply escapeEq, reflLRTyEq; [|tea].
 Qed.
 
+Lemma isLRFun_isWfFun : forall {σ Δ f} (wfΔ : [|- Δ]) (RΠFG : [Δ ||-< l > (tProd F G)[σ]])
+  (p : [Δ ||-Π f[σ] : tProd F[σ] G[up_term_term σ] | normRedΠ0 (Induction.invLRΠ RΠFG)]),
+  isWfFun Δ F[σ] G[up_term_term σ] (PiRedTm.nf p).
+Proof.
+intros.
+destruct RΠFG; simpl in *.
+destruct p as [nf ? isfun]; simpl in *.
+destruct isfun as [A t vA|]; simpl in *; constructor; tea.
+rewrite <- (wk_id_ren_on Δ F[σ]), <- (wk_id_ren_on Δ A).
+now unshelve eapply escapeEq, vA.
+Qed.
 
 Lemma ηeqEqTerm {σ Δ f g} (ρ := @wk1 Γ F)
   (Vfg : [Γ ,, F ||-v<l> tApp f⟨ρ⟩ (tRel 0) ≅ tApp g⟨ρ⟩ (tRel 0) : G | VΓF | VG ])
@@ -253,10 +266,11 @@ Proof.
   - change [Δ ||-<l> g[σ] : (tProd F G)[σ] | RΠ ]; irrelevance.
   - cbn; pose (VσUp :=  liftSubstS' VF Vσ).
     instValid Vσ; instValid VσUp; escape.
-    destruct (PiRedTm.red p); destruct (PiRedTm.red p0); cbn in *.
     eapply convtm_eta; tea.
-    + apply (PiRedTm.isfun p0).
-    + apply (PiRedTm.isfun p).
+    + destruct (PiRedTm.red p0); cbn in *; tea.
+    + now apply isLRFun_isWfFun.
+    + destruct (PiRedTm.red p); cbn in *; tea.
+    + now apply isLRFun_isWfFun.
     + etransitivity ; [symmetry| etransitivity]; tea; eapply ηeqEqTermConvNf.
   - match goal with H : [_ ||-Π f[σ] : _ | _] |- _ => rename H into Rfσ end.
     match goal with H : [_ ||-Π g[σ] : _ | _] |- _ => rename H into Rgσ end.
